\documentclass[10pt,a4paper,oneside]{article}

\usepackage{algorithm}
\usepackage{algpseudocode}
\usepackage{bigints}
\usepackage{graphicx}
\usepackage{epstopdf}
\usepackage[noblocks]{authblk}
\usepackage{amssymb}
\usepackage{amsmath}
\usepackage{amsfonts}
\usepackage{mathtools}
\usepackage{color}
\usepackage{listings}
\usepackage{fancyvrb}
\usepackage{float}
\usepackage{framed}
\usepackage{multirow}
%\usepackage{hyperref}
\usepackage{url}  % This makes \url work
\usepackage{multicol}
\usepackage{subcaption}
\setlength{\columnsep}{1cm}
\usepackage{pifont}
\usepackage{colortbl}
\usepackage{framed}
\usepackage{listings}
\usepackage{bm}
\usepackage{eurosym}
\usepackage{amssymb}% http://ctan.org/pkg/amssymb
\usepackage{suffix}
\usepackage{tikz}
\usepackage{bbm}
\usetikzlibrary{matrix}
\usepackage[customcolors]{hf-tikz}

\usepackage[toc,page]{appendix}

\newcommand{\cmark}{\ding{51}}%
\floatname{algorithm}{Procedure}
\renewcommand{\algorithmicrequire}{\textbf{Input:}}
\renewcommand{\algorithmicensure}{\textbf{Output:}}

\usepackage[a4paper,left=2cm,right=2cm,top=2.5cm,bottom=2.5cm]{geometry}

%%enviroments for Theorems, propositions
\newtheorem{theorem}{Theorem}[section]
\newtheorem{proposition}[theorem]{Proposition}
\newtheorem{assumption}[theorem]{Assumption}
\newtheorem{corollary}[theorem]{Corollary}
\newtheorem{definition}[theorem]{Definition}
\newtheorem{lemma}[theorem]{Lemma}
\newtheorem{remark}[theorem]{Remark}
\newtheorem{observation}[theorem]{Observation}
\newtheorem{problem}{Open Problem}[section]
\newtheorem{conjecture}{Conjecture}[section]
\newtheorem{example}[theorem]{Example}
\newenvironment{proof}{\noindent{\bf Proof:}}{\hfill$\square$}

\DeclareMathOperator{\arcsinh}{arcsinh}
\DeclareMathOperator{\erfc}{erfc}

\DeclarePairedDelimiter\ceil{\lceil}{\rceil}
\DeclarePairedDelimiter\floor{\lfloor}{\rfloor}
\newcommand\numberthis{\addtocounter{equation}{1}\tag{\theequation}}


\title{On the computation and inversion of the Normal Inverse Gaussian cumulative distribution function}
\author{
 \normalsize  Guillermo Navas-Palencia\\
  \texttt{\normalsize  g.navas.palencia@gmail.com}
}

\date{\small \today}

\begin{document}
\maketitle

\tableofcontents
\newpage
\section{Introduction}

Variance-mean mixture distribution
\begin{equation}
Z \sim \mathcal{IG}(\delta \gamma, \gamma^2), \quad X \sim \mathcal{N}(\mu + \beta Z, Z),
\end{equation}
where $\gamma = \sqrt{\alpha^2 - \beta^2}$. The domain of the parameters is
\begin{equation}
0 \le |\beta| < \alpha, \quad \mu \in \mathbb{R}, \quad \delta  > 0.
\end{equation}

The density function is given by
\begin{equation}
f(x; \alpha, \beta, \mu, \delta) = \frac{\alpha \delta}{\pi} \frac{K_1\left(\alpha\sqrt{\delta^2 + (x-\mu)^2}\right)}{\sqrt{\delta^2 + (x-\mu)^2}} e^{\delta \gamma + \beta(x-\mu)}
\end{equation}

The cumulative distribution function is given by
\begin{equation}\label{integral_k1}
F(x; \alpha, \beta, \mu, \delta) = \frac{\alpha \delta e^{\delta \gamma}}{\pi} \int_{-\infty}^{x} \frac{K_1\left(\alpha\sqrt{\delta^2 + (t-\mu)^2}\right)}{\sqrt{\delta^2 + (t-\mu)^2}} e^{\beta(t-\mu)} \mathop{dt}
\end{equation}

\begin{equation}\label{integral_phi}
F(x; \alpha, \beta, \mu, \delta) = \frac{\delta}{\sqrt{2\pi}}\int_{0}^{\infty} \Phi\left(\frac{x - (\mu +\beta t)}{\sqrt{t}}\right) t^{-3/2} e^{-\frac{(\delta - \gamma t)^2}{2t}} \mathop{dt}
\end{equation}

\paragraph{Integral representations}

\begin{proposition} Because $|\beta| < \alpha$, we can write $\beta = \alpha \tanh(\theta)$. Substituting in \eqref{integral_k1} $x-\mu = \delta \sinh(\theta + u)$ we obtain
\begin{equation}
F(x; \alpha, \beta, \mu, \delta) = \frac{\alpha \delta e^{\delta \gamma}}{\pi} \int_{-\infty}^{\tau} K_1 \left(\alpha \delta \cosh(\theta + u)\right) e^{\beta \delta \sinh(\theta + u)} \mathop{du},
\end{equation}
where
\begin{equation}
\tau = \arcsinh\left(\frac{x - \mu}{\delta}\right) - \theta.
\end{equation}

\end{proposition}

\paragraph{Standard case $\mu = 0$ and $\delta = 1$}
\paragraph{Case $\mu = 0$}
\paragraph{Case $\delta = 0$}
\paragraph{Case $x=\mu$}

If $x = \mu$ and $\beta = 0$ then $F(x; \alpha, 0, \mu, \delta) = \frac{1}{2}$.

\section{Preliminaries}

In this section, we present some results to be used throughout this work.

\subsection{The function $\Phi\left(\frac{a}{\sqrt{t}} + b\sqrt{t}\right)$}

The function $F(t; a, b) = \Phi\left(\frac{a}{\sqrt{t}} + b\sqrt{t}\right)$ is part of the integrand of the integral representation in \eqref{integral_phi}. Given its relevance throughout this work, we introduce here some results that shall be used subsequently. $F(t; a, b)$ has the following integral representation \cite[\S 7.7.6]{NIST:DLMF}
\begin{equation}\label{integral_erfc_ab}
F(t; a, b) = \frac{1}{2}\erfc\left(-\frac{\frac{a}{\sqrt{t}} + b\sqrt{t}}{\sqrt{2}}\right)  = \sqrt{\frac{t}{\pi}} e^{-\frac{a^2}{2t}} \int_{-b/\sqrt{2}}^{\infty} e^{-(tu^2 - \sqrt{2}au)} \mathop{du}
\end{equation}

\subsubsection{Expansion $t \to 0$}

Let us consider the case $a < 0$, since we can use the mirror property $\Phi(z) = 1 - \Phi(-z)$ otherwise. To obtain an expansion for $t \to 0$, we expand $e^{-tu^2}$ and interchange summation and integration obtaining
\begin{equation*}
F(t; a, b) = \sqrt{\frac{t}{\pi}} e^{-\frac{a^2}{2t}} \sum_{k=0}^{\infty} \frac{(-t)^k}{k!}\int_{-b/\sqrt{2}}^{\infty} e^{\sqrt{2}a u} u^{2k}\mathop{du}.
\end{equation*}
For $a < 0$ the integral can be expressed in closed-form in terms of the incomplete gamma function, $\Gamma(a, x)$
\begin{equation*}
\int_{-b/\sqrt{2}}^{\infty} e^{\sqrt{2}a u} u^{2k}\mathop{du} = \frac{\Gamma(2k+1, -ab)}{(\sqrt{2}a)^{2k+1}},
\end{equation*}
and for the special case $b=0$, it reduces to
\begin{equation*}
\int_{0}^{\infty} e^{\sqrt{2}a u} u^{2k}\mathop{du} = \frac{\Gamma(2k+1)}{(\sqrt{2}a)^{2k+1}}.
\end{equation*}
Then, we obtain the series expansion valid for $t \to 0$, $a \to -\infty$ and fixed $b$
\begin{equation}
F(t; a, b) = \sqrt{\frac{t}{\pi}} e^{-\frac{a^2}{2t}} \sum_{k=0}^{\infty} \frac{(-1)^{k+1} t^k}{k!}\frac{\Gamma(2k + 1, ab)}{(\sqrt{2}a)^{2k+1}}.
\end{equation}

Moreover, another expansion valid for large values of $a > 0$ and $b$ can be obtained after expanding $F(t;a,b)$ at $t=0$. The first coefficients are
\begin{equation}
c_0 = \frac{1}{a}, \quad c_1 = \frac{ab + 1}{a^3}, \quad c_2 = \frac{a^2bÂ² +3ab + 3}{a^5}, \quad c_3 = \frac{a^3b^3 + 6a^2b^3 + 15ab + 15}{a^7}
\end{equation}
and the expansion reads
\begin{equation}
F(t; a, b) = 1 + \frac{e^{-\frac{1}{2} \left(\frac{a}{\sqrt{t}} + b\sqrt{t} \right)^2}}{\sqrt{2\pi}}\sum_{k=0}^{\infty}(-1)^{k+1}c_k t^{k + \frac{1}{2}}.
\end{equation}
The coefficients are expressible in terms of Bessel polynomials $y_k(x)$ \cite[\S A001498]{OEIS}, and it follows that
\begin{equation}
F(t; a, b) = 1 + \frac{e^{-\frac{1}{2} \left(\frac{a}{\sqrt{t}} + b\sqrt{t} \right)^2}}{a\sqrt{2\pi}}\sum_{k=0}^{\infty}(-1)^{k+1} \left(\frac{b}{a}\right)^k y_k\left(\frac{1}{ab}\right) t^{k + \frac{1}{2}},
\end{equation}
where $y_k(x)$ has an explicit formula
\begin{equation}
y_k(x) = \sum_{m=0}^k \binom{k}{m} (k + 1)_m \left(\frac{x}{2}\right)^m.
\end{equation}

Using the connection of the Bessel polynomials with the modified Bessel function of the second kind $K_k(x)$ given by \cite[\S 33.1.3]{Temme2015}
\begin{equation}
y_k(x) = \sqrt{\frac{2}{\pi x}}e^{1/x} K_{k + \frac{1}{2}}\left(\frac{1}{x}\right),
\end{equation}
the resulting expansion is represented as a Bessel-type expansion
\begin{equation}
F(t; a, b) = 1 + \frac{e^{-\frac{a^2}{2t} - \frac{b^2}{2}t}}{\pi}\sqrt{\frac{b}{a}}\sum_{k=0}^{\infty} (-1)^{k+1} \left(\frac{b}{a}\right)^k K_{k + \frac{1}{2}}(ab)t^{k + \frac{1}{2}}.
\end{equation}
The expansion is convergent for $t < 1$. The convergence follows from the asymptotic estimate of $(b/a)^k K_k(ab) \sim (b/a)^k \sqrt{\frac{\pi}{2ab}}e^{-ab}$ as $|ab| \to \infty$. The expansion can be seen as an asymptotic expansion for large $a$, or as a uniform asymptotic expansion for $a \sim b$. The coefficients can be computed by using a recurrence relation for the modified Bessel function.

\subsubsection{Expansion $t \to \infty$}

Let us focus on the case $t \to \infty$. We can develop an asymptotic expansion after expanding the term $e^{\sqrt{2}au}$ in \eqref{integral_erfc_ab}, which yields
\begin{equation*}
F(t; a, b) = \sqrt{\frac{t}{\pi}} e^{-\frac{a^2}{2t}} \sum_{k=0}^{\infty}\frac{(\sqrt{2}a)^k}{k!}\int_{-b/\sqrt{2}}^{\infty} e^{-t u^2} u^k \mathop{du}.
\end{equation*}
Considering the case $b < 0$ (again, we can use the mirror property), the integral has a closed-form
\begin{equation*}
\int_{-b/\sqrt{2}}^{\infty} e^{-t u^2} u^k \mathop{du} = \frac{\Gamma\left(\frac{k+1}{2}, \frac{b^2}{2}t\right)}{2 t^{\frac{k+1}{2}}}.
\end{equation*}
Thus,
\begin{equation}\label{phi_expansion_incgamma}
F(t; a, b) = \sqrt{\frac{t}{\pi}} \frac{e^{-\frac{a^2}{2t}}}{2}  \sum_{k=0}^{\infty}\frac{(\sqrt{2}a)^k}{k!} \frac{\Gamma\left(\frac{k+1}{2}, \frac{b^2}{2}t\right)}{t^{\frac{k+1}{2}}}.
\end{equation}
The asymptotic behaviour of the terms in the series is
\begin{equation*}
\frac{\Gamma\left(\frac{k+1}{2}, \frac{b^2}{2}t\right)}{t^{\frac{k+1}{2}}} \sim \left(\frac{b^2}{2}\right)^{\frac{k+1}{2}} e^{-\frac{b^2}{2} t}, \quad t\to\infty.
\end{equation*}
In fact this series is convergent, as can be observed taking the asymptotic estimate of $\Gamma(k, x)$ as $k \to \infty$. A simpler convergent expansion can be obtained transforming the integral in \eqref{integral_erfc_ab}
\begin{equation*}
\sqrt{\frac{t}{\pi}} e^{-\frac{a^2}{2t}} \int_{-b/\sqrt{2}}^{\infty} e^{-(tu^2 - \sqrt{2}au)} \mathop{du} = \sqrt{\frac{t}{\pi}} e^{-\frac{a^2}{2t} -ab - \frac{b^2}{2}t}\int_0^{\infty}e^{\sqrt{2}(a+bt)u} e^{-tu^2}\mathop{dt},
\end{equation*}
and expanding $e^{\sqrt{2}(a+bt)u}$ obtaining
\begin{equation}
F(t; a, b) = \sqrt{\frac{t}{\pi}} \frac{e^{-\frac{a^2}{2t} -ab - \frac{b^2}{2}t}}{2} \sum_{k=0}^{\infty} \frac{(\sqrt{2}(a+bt))^k}{k!}\frac{\Gamma\left(\frac{k+1}{2}\right)}{t^{\frac{k+1}{2}}}.
\end{equation}

Similarly to the expansion at $t \to 0$, we can obtain an asymptotic expansion expanding $F(t; a, b)$ at $t \to \infty$. For $b > 0$, the first terms of the expansion are
\begin{equation}
c_0 = 1, \quad c_1 = 2 + 2ab + a^2 b^2, \quad c_2 = 24 + 24ab + 12a^2b^2 + 4a^3b^3 + a^4b^4,
\end{equation}
\begin{equation}
F(t; a, b) = 1 + \frac{e^{-ab - \frac{b^2}{2}t}}{\sqrt{2\pi}}\sum_{k=0}^{\infty}\frac{(-1)^{k+1}}{2^k k!}\frac{c_k}{b^{2k+1}}\left(\frac{1}{t}\right)^{k+\frac{1}{2}}.
\end{equation}
The coefficients $c_k$ are expressible in terms of the incomplete gamma function, since
\begin{equation*}
c_k = \sum_{j=0}^{2k}\frac{(2k)!}{j!}(ab)^j = e^{ab}\Gamma(2k+1, ab).
\end{equation*}
Rearranging terms, we get
\begin{equation}
F(t; a, b) = 1 + \frac{e^{- \frac{b^2}{2}t}}{\sqrt{2\pi}}\sum_{k=0}^{\infty}\frac{(-1)^{k+1}}{2^k k!}\frac{\Gamma(2k+1, ab)}{b^{2k+1}}\left(\frac{1}{t}\right)^{k+\frac{1}{2}}.
\end{equation}

\subsubsection{Expansion $t \to u$}

Lastly, we study the expansion of $F(t;a,b)$ at $t=u$. This expansion shall be crucial when developing various Bessel-type asymptotic expansions later on. The first coefficients of the Taylor series are
\begin{equation*}
c_0 = \Phi\left(\frac{a}{\sqrt{u}} + b\sqrt{u}\right)d_0,\quad c_1 = \phi\left(\frac{a}{\sqrt{u}} + b\sqrt{u}\right) d_1, \quad c_2 = -\phi\left(\frac{a}{\sqrt{u}} + b\sqrt{u}\right) d_2, \quad
c_3 = \phi\left(\frac{a}{\sqrt{u}} + b\sqrt{u}\right) d_3,
\end{equation*}
where
\begin{align*}
d_0 &= 1\\
d_1 &= \frac{-a + bu}{2u^{3/2}}\\
d_2 &=\frac{a^3 -3au -a^2 bu + bu^2 -ab^2 u^2 + b^3u^3}{8 u^{7/2}}\\
d_3 &= \frac{-a^5 +10a^3u + a^4bu -15au^2 - 6a^2bu^2 + 2a^3 b^2 u^2 +3bu^3 -6ab^2u^3 - 2a^2b^3 u^3 + 2b^3 u^4 -ab^4u^4 + b^5 u^5}{48 u^{11/2}},
\end{align*}
and $\phi(x) = \frac{e^{-x^2/2}}{\sqrt{2\pi}}$ is the probability density function of the standard normal distribution. Thus, we have
\begin{equation}
F(t; a, b) = \sum_{k=0}^{\infty} c_k (t-u)^k.
\end{equation}
Additional terms satisfy the following recurrence
\begin{equation}
c_{k+4} = \frac{f_0(k) c_k + f_1(k) c_{k+1} + f_2(k) c_{k+2} + f_3(k) c_{k+3}}{f_4(k)}, \quad k \ge 0
\end{equation}
where
\begin{align*}
f_0(k) &= -kb^3\\
f_1(k) &= -(1 + k) b (1 + 2k -ab + 3b^3u)\\
f_2(k) &= (2 + k)(5a + 2ka +a^2b - 8bu - 6kbu +2ab^2u -3b^3u^2)\\
f_3(k) &= -(3 + k)(a^3 - 11au -4kau - a^2bu + 13bu^2 + 6kbu^2 -ab^2u^2 + b^3 u^3)\\
f_4(k) &= 2 (3 + k) (4 + k) u^2 (-a + bu)
\end{align*}

\subsection{Bessel-type expansions}

\section{Methods of computation}
\subsection{Expansions $|x-\mu| \to 0$}
The starting point is the integral representation in \eqref{integral_phi} after expanding the exponential
\begin{equation*}
F(x;\alpha, \beta, \mu, \delta) = \frac{\delta e^{\delta \gamma}}{\sqrt{2\pi}} \int_{0}^{\infty} \Phi\left(\frac{x - (\mu +\beta t)}{\sqrt{t}}\right) t^{-3/2} e^{-\frac{\delta^2}{2t} - \frac{\gamma^2}{2}t} \mathop{dt},
\end{equation*}
and replacing $\Phi\left(\frac{x - (\mu +\beta t)}{\sqrt{t}}\right)$ by the expansion in \eqref{phi_expansion_incgamma}
\begin{equation*}
F(x;\alpha, \beta, \mu, \delta) = \frac{\delta e^{\delta \gamma}}{\sqrt{2\pi}} \sum_{k=0}^{\infty}\frac{2^{k/2}(x-\mu)^k}{k!}\int_0^{\infty}\Gamma\left(\frac{k+1}{2}, \frac{\beta^2}{2}t\right) t^{-3/2-k/2} e^{-\frac{\omega^2}{2t} - \frac{\gamma^2}{2}t} \mathop{dt},
\end{equation*}
where $\omega = \sqrt{\delta^2 + (x-\mu)^2}$. Consider the ascending series of the incomplete gamma function given by \cite[\S 8.7]{NIST:DLMF}
\begin{equation}
\Gamma(a, x) = \Gamma(a) - \sum_{j=0}^{\infty} \frac{(-1)^j x^{a+j}}{j! (a+ j)}.
\end{equation}
We proceed splitting the inner integral into two terms
\begin{align}
T_1 &= \Gamma\left(\frac{k+1}{2}\right)\int_0^{\infty}t^{-3/2-k/2} e^{-\frac{\omega^2}{2t} - \frac{\gamma^2}{2}t} \mathop{dt}\\
T_2 &= \sum_{j=0}^{\infty} \frac{(-1)^j \left(\frac{\beta^2}{2}\right)^{\frac{k+1}{2}+j}}{j! (\frac{k+1}{2}+ j)}\int_0^{\infty} t^{j-1} e^{-\frac{\omega^2}{2t} - \frac{\gamma^2}{2}t} \mathop{dt},
\end{align}
and observe that both integrals are expressible in terms of modified Bessel function, resulting in the sums $S_1$ and $S_2$, such that $F(x;\alpha, \beta, \mu, \delta) = C (S_1 - S2)$, defined as follows
\begin{align}
S_1 &= \sum_{k=0}^{\infty}\frac{2^{k/2}(x-\mu)^k}{k!} \Gamma\left(\frac{k+1}{2}\right)2 K_{\frac{k+1}{2}}(\omega \gamma) \left(\frac{\gamma}{\omega}\right)^{\frac{k+1}{2}}\\
S_2 &= \sum_{k=0}^{\infty}\frac{2^{k/2}(x-\mu)^k}{k!}\sum_{j=0}^{\infty}\frac{(-1)^j \left(\frac{\beta^2}{2}\right)^{\frac{k+1}{2}+j}}{j! (\frac{k+1}{2}+ j)} 2 K_j(\omega \gamma) \left(\frac{\omega}{\gamma}\right)^j.
\end{align}
Interchanging the order of summation in $S_2$, we observe that the sum in $k$ is convergent an expressible in terms of the lower incomplete gamma function $\gamma(a, x)$. Assuming $\beta > 0$
\begin{equation}
\sum_{k=0}^{\infty}\frac{2^{k/2}(x-\mu)^k}{k! (\frac{k+1}{2}+ j)} \left(\frac{\beta^2}{2}\right)^{\frac{k+1}{2}} = -\frac{\sqrt{2}}{(x-\mu)^{2j+1}\beta^{2j}} \gamma \left(2j + 1, -(x-\mu)\beta\right).
\end{equation}
Thus,
\begin{equation*}
S_2 = -2\sqrt{2} \sum_{j=0}^{\infty} \frac{(-1)^j}{j!}\frac{\gamma \left(2j + 1, -(x-\mu)\beta\right)}{(x-\mu)^{2j+1}\beta^{2j}} \left(\frac{\beta^2}{2}\right)^j  K_j(\omega \gamma) \left(\frac{\omega}{\gamma}\right)^j
\end{equation*}
Rearranging terms
\begin{align}
F(x;\alpha, \beta, \mu, \delta) = \frac{\delta e^{\delta \gamma}}{\pi \sqrt{2}} \bigg[& \sum_{k=0}^{\infty}\frac{2^{k/2}(x-\mu)^k}{k!} \Gamma\left(\frac{k+1}{2}\right) K_{\frac{k+1}{2}}(\omega \gamma) \left(\frac{\gamma}{\omega}\right)^{\frac{k+1}{2}}\nonumber\\
& + \sqrt{2}\sum_{k=0}^{\infty} \frac{(-1)^k}{k!}\frac{\gamma \left(2k + 1, -(x-\mu)\beta\right)}{(x-\mu)^{2k+ 1}}  K_k(\omega \gamma) \left(\frac{\omega}{2\gamma}\right)^k \bigg]
\end{align}

If $\beta < 0$ then $F(x;\alpha, \beta, \mu, \delta) = 1 - F(-x;\alpha, -\beta, -\mu, \delta)$. The expansion is convergent for small $x-\mu$ and fixed values of the rest of parameters. Moreover, the convergence improves when $\gamma \sim \omega$, also valid for large values for these two parameters.

\subsubsection{Case $\delta \to \infty$}


\subsubsection{Special value $\beta = 0$}

We use the integral \eqref{integral_phi}. For $|x - \mu| \to 0$, we use the series expansion of $\Phi(x)$ given by

\begin{equation*}
\Phi(x) = \frac{1}{2} + \frac{1}{\sqrt{2\pi}}\sum_{k=0}^{\infty} \frac{(-1)^k x^{2k + 1}}{2^k k! (2k+1)}
\end{equation*}

\begin{equation*}
\Phi(x) = \frac{1}{2} + \frac{e^{-x^2 / 2}}{\sqrt{2\pi}}\sum_{k=0}^{\infty} \frac{x^{2k+1}}{(2k + 1)!!}
\end{equation*}

Use closed-form in terms of the modified Bessel function. Alternating series
\begin{equation}
F(x; \alpha, 0, \mu, \delta) = \frac{1}{2} + \frac{\delta e^{\delta \gamma}}{\pi}\sum_{k=0}^{\infty} \frac{(-1)^k (x-\mu)^{2k+1}}{2^k k! (2k + 1)} \left(\frac{\alpha}{\delta}\right)^{k+1}K_{k+1}(\alpha \delta).
\end{equation}
Asymptotic analysis of $K_{k+1}(\alpha \delta)$. To obtain a series with positive term for $x - \mu > 0$, use alternative expansion of $\Phi(x)$

\begin{equation}
F(x; \alpha, 0, \mu, \delta) = \frac{1}{2} + \frac{\delta e^{\delta \gamma}} {\pi}\sum_{k=0}^{\infty} \frac{(x-\mu)^{2k+1}}{(2k +1)!!} \left(\frac{\alpha}{\omega}\right)^{k+1}K_{k+1}(\alpha \omega), \quad \omega = \sqrt{\delta^2 + (x-\mu)^2}.
\end{equation}


\subsection{Expansion $\alpha \to \infty, \delta \to \infty$}

\subsection{Expansion $|x-\mu| \to \infty$}

The expansion of $\Phi\left(\frac{x-(\mu + \beta t)}{\sqrt{t}}\right)$ at $t\to 0$ is given in terms of the Bessel polynomial $y_k(x)$. To simplify notation, we take $a = x-\mu$ and $b=-\beta$. Then,

\begin{equation}
\Phi\left(\frac{a}{\sqrt{t}} + b\sqrt{t}\right) = 1 + \frac{e^{-a^2/(2t) -ab - b^2/2 t}}{a\sqrt{2\pi}}\sum_{k=0}^{\infty} (-1)^{k+1} \left(\frac{b}{a}\right)^k y_k\left(\frac{1}{ab}\right) t^{\frac{1}{2} + k}
\end{equation}

Using the connection of the Bessel polynomials with the modified Bessel function of the second kind $K_n(x)$ given by
\begin{equation}
y_n(x) = \sqrt{\frac{2}{\pi x}}e^{1/x} K_{n + \frac{1}{2}}\left(\frac{1}{x}\right),
\end{equation}
we replace in the integral, we obtain
\begin{equation}
F(x; \alpha, \beta, \mu, \delta) = 1 + \delta e^{\delta \gamma} \sqrt{\frac{b}{2a\pi^3}}\sum_{k=0}^{\infty} (-1)^{k+1} \left(\frac{b}{a}\right)^k K_{k + \frac{1}{2}}(ab)\int_0^{\infty}t^{k-1} e^{-\frac{\delta^2 + a^2}{2t} -\frac{\gamma^2 + b^2}{2}t} \mathop{dt}
\end{equation}

\begin{equation}
\int_0^{\infty}t^{k-1} e^{-\frac{\delta^2 + a^2}{2t} -\frac{\gamma^2 + b^2}{2}t} \mathop{dt} = 2 K_k(\omega \alpha) \left(\frac{\omega}{\alpha}\right)^k,
\end{equation}
where $\omega = \sqrt{\delta^2 + (x-\mu)^2}$. Rearranging terms
\begin{equation}
F(x; \alpha, \beta, \mu, \delta) = 1 + \delta e^{\delta \gamma} \sqrt{\frac{2\beta}{(\mu-x)\pi^3}}\sum_{k=0}^{\infty} (-1)^{k+1} \left(\frac{\beta \omega}{\alpha(\mu-x)}\right)^k K_{k + \frac{1}{2}}((\mu-x)\beta) K_k(\omega \alpha) 
\end{equation}

\section{Other expansions}

\begin{proposition} For $x - \mu < 0$
\begin{equation}\label{integral_k0}
F(x; \alpha, \beta, \mu, \delta) = \frac{\sqrt{2}\delta e^{\delta \gamma}}{\pi}\int_{\beta / \sqrt{2}}^{\infty} e^{\sqrt{2}(x-\mu)t} K_0\left(\sqrt{2\left( (x-\mu)^2 + \delta^2\right)} \sqrt{\frac{\gamma^2}{2} + t^2}\right) \mathop{dt}
\end{equation}
\end{proposition}
\begin{proof}
Consider the integral representation of the function $\Phi\left(\frac{x-\mu}{\sqrt{t}} -\beta \sqrt{t} \right)$
\begin{equation*}
\Phi\left(\frac{x-\mu}{\sqrt{t}} -\beta \sqrt{t} \right) = \sqrt{\frac{t}{\pi}} e^{-\frac{(x-\mu)^2}{2t}}\int_{\beta/\sqrt{2}}^{\infty} e^{-(tu^2 - \sqrt{2}(x-\mu) u)} \mathop{du}.
\end{equation*}
Replacing in \eqref{integral_phi} and interchanging the order of integration we obtain
\begin{equation*}
F(x; \alpha, \beta, \mu, \delta) = \frac{\delta e^{\delta \gamma}}{\sqrt{2}\pi} \int_{\beta/\sqrt{2}}^{\infty} e^{\sqrt{2}(x-\mu) u} \int_{0}^{\infty} t^{-1} e^{-\frac{\left((x-\mu)^2 + \delta^2\right)}{2t} - \left(\frac{\gamma^2}{2} + u^2\right)t} \mathop{dt} \mathop{du}.
\end{equation*}
The observation that the inner integral can be represented in terms of the modified Bessel function $K_0$
\begin{equation*}
\int_{0}^{\infty} t^{-1} e^{-\frac{\left((x-\mu)^2 + \delta^2\right)}{2t} - \left(\frac{\gamma^2}{2} + u^2\right)t} \mathop{dt} = 2 K_0\left(2\sqrt{\frac{(x-\mu)^2 + \delta^2}{2}} \sqrt{\frac{\gamma^2}{2} + t^2}\right).
\end{equation*}
\end{proof}

A similar expansion can be obtained from the integral representation \eqref{integral_k0}, expanding $e^{\sqrt{2}(x-\mu)t}$
\begin{equation*}
e^{\sqrt{2}(x-\mu)t} = \sum_{k=0}^{\infty} \frac{2^{k/2} (x-\mu)^k}{k!} t^k
\end{equation*}

\begin{equation*}
F(x; \alpha, 0, \mu, \delta) = \frac{\sqrt{2}\delta e^{\delta \gamma}}{\pi} \sum_{k=0}^{\infty} \frac{2^{k/2} (x-\mu)^k}{k!} \int_{0}^{\infty} t^k K_0\left(\sqrt{2\left( (x-\mu)^2 + \delta^2\right)} \sqrt{\frac{\gamma^2}{2} + t^2}\right) \mathop{dt}
\end{equation*}
Use closed-form in terms of the modified Bessel function
\begin{equation}
F(x; \alpha, 0, \mu, \delta) = \frac{\delta e^{\delta \gamma}}{2\pi} \sum_{k=0}^{\infty} \frac{(x-\mu)^k}{2^{k/2} \Gamma\left(\frac{k}{2} + 1\right)}\left(\frac{\alpha}{\omega}\right)^{\frac{k+1}{2}}K_{\frac{k+1}{2}}(\omega \alpha), \quad \omega = \sqrt{\delta^2 + (x-\mu)^2}.
\end{equation}


\section{Inversion methods}

\section{Numerical experiments}



\bibliographystyle{plain}
\bibliography{bib}

\end{document}
